## 最优化理论第一次作业

22336226

王泓沣



1. 证明：

$\because C\subseteq R^n$ 为一个凸集

$\therefore\forall x_1,x_2\in C,\forall \theta_1,\theta_2\in \mathbb{R}\space s.t. \theta_1+\theta_2=1,\theta_1,\theta_2\geqslant0$ 有 $\theta_1x_1+\theta_2x_2\in C$  

$\therefore\exist u_1\in C, u_1=\theta_1x_1+\theta_2x_2$

$\therefore\forall x_3\in C,\forall\theta_1,\theta_2\in\mathbb{R}\space s.t. \theta_1+\theta_2=1\therefore \theta_3 u_1+\theta_4x_3\in C$

依此类推，得证



2. 证明：

$$
\begin{aligned}
&\forall x_1,x_2\in C,\forall \theta_1,\theta_2\in R\space s.t. \theta_1+\theta_2=1,\theta_1,\theta_2\geqslant0\\
&A(\theta_1x_1+\theta_2x_2)=\theta_1Ax_1+\theta_2Ax_2=b_1+b_2\\
&\therefore\theta_1x_1+\theta_2x_2\in C\\
&\therefore C为凸集
\end{aligned}
$$



3. 证明：

$$
\begin{aligned}
\forall &x_1,x_2\in\mathbb{R}^n,\forall\theta_1,\theta_2\in\mathbb{R}\geqslant0\space s.t.\theta_1+\theta_2=1,\\
令s=&(\theta_1x_1+\theta_2x_2)^\top A(\theta_1x_1+\theta_2x_2)+b^\top (\theta_1x_1+\theta_2x_2)+c\\ 
=& \theta_1^2x_1^\top Ax_1+\theta_1\theta_2x_2^\top A x_1+\theta_1\theta_2x_1^\top Ax_2+\theta_2^2x_2^\top Ax_2+\theta_1b^\top x_1+\theta_2b^\top x_2+c\\
\because\space &A\succeq0\\
\therefore\space &x_1^\top Ax_2=x_2^\top Ax_1\\
令\lambda_1=&\theta_1(x_1^\top A x_1+b^\top x_1+c),\lambda_2=\theta_2(x_2^\top Ax_2+b^\top x_2+c) \\
s-\lambda_1-\lambda_2&=(\theta_1^2-\theta_1)x_1^\top A x_1+2\theta_1\theta_2x_1^\top Ax_2+(\theta_2^2-\theta_2)x_2^\top Ax_2\\
&=-\theta_1\theta_2(x_1-x_2)^\top A(x_1-x_2)\\
\because &\space A\succeq0\\
\therefore &\space-\theta_1\theta_2(x_1-x_2)^\top A(x_1-x_2)\leqslant0\\
\because &\space\lambda_1\leqslant0,\lambda_2\leqslant0\\
\therefore &\space s\leqslant0\\
\therefore &\space \theta_1x_1+\theta_2x_2\in C\\
\therefore &\space C是凸集
\end{aligned}
$$



4. 解：

（a）
$$
\begin{aligned}
\bigtriangledown&^2 f(x)=\sum^n_{i=1}\frac{1}{x_i}\\
\because\space &x_i\in\mathbb{R}_{++}\\
\therefore\space &\bigtriangledown^2f(x)\succ0\\
\therefore\space &f(x)为严格凸函数
\end{aligned}
$$
（b）
$$
\begin{aligned}
\dfrac{\partial f}{\partial x_1}&=x_2\\
\dfrac{\partial f}{\partial x_2}&=x_1\\
\dfrac{\partial^2f}{\partial x_1^2}&=0\\
\dfrac{\partial^2f}{\partial x_2^2}&=0\\
\dfrac{\partial^2f}{\partial x_1\partial x_2}&=1\\
\dfrac{\partial^2f}{\partial x_2\partial x_1}&=1\\
\therefore Hessian矩阵&为
\left[
\begin{matrix}
0&1\\
1&0\\
\end{matrix}
\right]
\\
\therefore \lambda_1 = -1&,\lambda_2=1\\
\therefore f(x_1,x_2)&为非凸非凹函数
\end{aligned}
$$
（c）
$$
\begin{aligned}
\dfrac{\partial f}{\partial x_1}&=\dfrac{1}{x_2}\\
\dfrac{\partial f}{\partial x_2}&=-\dfrac{x_1}{x_2^2}\\
\dfrac{\partial^2f}{\partial x_1^2}&=0\\
\dfrac{\partial^2f}{\partial x_2^2}&=\dfrac{2x_1}{x_2^3}\\
\dfrac{\partial^2f}{\partial x_1\partial x_2}&=-\dfrac{1}{x_2^2}\\
\dfrac{\partial^2f}{\partial x_2\partial x_1}&=-\dfrac{1}{x_2^2}\\
\therefore Hessian矩阵&为
\left[
\begin{matrix}
0&-\dfrac{1}{x_2^2}\\
-\dfrac{1}{x_2^2}&\dfrac{2x_1}{x_2^3}\\
\end{matrix}
\right]
\\
\lambda^2-\dfrac{2x_1}{x_2^3}\lambda-\dfrac{1}{x_2^4}&=0\\
\lambda_1,\lambda_2&=\dfrac{\dfrac{2x_1}{x_2^3}\pm\sqrt{\dfrac{4x_1^2}{x_2^6}+\dfrac{4}{x_2^4}}}{2}\\
\therefore f(x_1,x_2)&是非凸非凹函数\\
\end{aligned}
$$


5. 证明：

$$
\begin{aligned}
&f(\theta x+(1-\theta )y)=h(g(\theta x+(1-\theta)y))\\
\because& g_i为凹函数\\
\therefore& g(\theta x+(1-\theta)y)\geqslant \theta g(x)+(1-\theta)g(y)\\
\because& h关于其每个分量非增\\
\therefore& h(g(\theta x+(1-\theta)y))\leqslant h(\theta g(x)+(1-\theta)g(y))\\
\because& h为凸函数\\
\therefore& h(\theta g(x)+(1-\theta)g(y))\leqslant \theta h(g(x))+(1-\theta)h(g(y))\\
即&f:=h\circ g为凸函数
\end{aligned}
$$

